\documentclass{article}

\usepackage[margin=1.0in]{geometry}
\usepackage{amsmath}
\usepackage{lmodern}

\begin{document}

\section{Dewar General Solution with Bdy-2 Applied}

\begin{equation}
\begin{split}
    \hat{\psi}(x,y) &= \left[-\overline{\psi}\cos{\mu a} + d_0\sin{\mu a} \right] \cos\left( \mu a \alpha \cos\left( \frac{my}{a} \right)  \right) \\
                    &+ \left[-\overline{\psi}\sin{\mu a} - d_0\cos{\mu a} \right] \sin\left( \mu a \alpha \cos\left( \frac{my}{a} \right)  \right) \\
                    &+i \sum_{l=1}^{\infty} d_{lm} \cos\left( \frac{lmy}{a} \right) \left[\sin\left( k_x^{(l)} a \right) \cos\left( k_x^{(l)}a \alpha \cos\left( \frac{my}{a} \right)  \right) \right]
\end{split}
\end{equation}

where $\left( k_x^{(l)} \right)^{2}=\mu^2 - \left( \frac{lm}{a} \right) ^2.$ Applying the following relations,

\begin{equation}
    \cos\left( z\cos\theta \right)=J_0\left( z \right) + 2 \sum_{k=1}^{\infty} (-1)^k J_{2k} \left( z \right) \cos\left( 2k\theta \right) 
\end{equation}
\begin{equation}
\sin\left(z\cos\theta\right)=2\sum_{k=0}^{\infty}(-1)^{k}J_{2k+1}\left(z\right)\cos\left((2k+1)\theta\right)
\end{equation} 

we get

\begin{equation}
    \begin{split}
        \hat{\psi}(x,y) &= \left[-\overline{\psi}\cos{\mu a} + d_0\sin{\mu a} \right] \\
                        &\left( J_0\left( \mu a \alpha \right) + 2 \sum_{n=1}^{\infty} (-1)^n J_{2n} \left( \mu a \alpha \right) \cos\left( \frac{2nmy}{a} \right) \right) \\
                        &+ \left[-\overline{\psi}\sin{\mu a} - d_0\cos{\mu a} \right] \\
                        &\left( 2\sum_{n=0}^{\infty}(-1)^{n}J_{2n+1}\left(\mu a \alpha \right)\cos\left( \frac{(2n+1)my}{a}\right) \right) \\
                        &+i \sum_{l=1}^{\infty} d_{lm}\sin\left( k_x^{(l)} a \right) \cos\left( \frac{lmy}{a} \right) \\
                        &\left[ J_0\left( k_x^{(l)} a \alpha \right) + 2 \sum_{n=1}^{\infty} (-1)^n J_{2n} \left( k_x^{(l)} a \alpha \right) \cos\left( \frac{2nmy}{a} \right) \right] \\
                        &-i \sum_{l=1}^{\infty} d_{lm}\cos\left( k_x^{(l)} a \right) \cos\left( \frac{lmy}{a} \right) \\
                        &\left[ 2\sum_{n=0}^{\infty}(-1)^{n}J_{2n+1}\left( k_x^{(l)  } a \alpha \right)\cos\left( \frac{(2n+1)my}{a}\right) \right]
    \end{split}
\end{equation} 

\newpage
which can be rearranged as

\begin{equation}
    \label{eq:eq64bdy2mode}
    \begin{split}
        \hat{\psi}(x,y) = J_0\left( \mu a \alpha \right)\left(-\overline{\psi}\cos{\mu a} + d_0\sin{\mu a} \right)& \\
        + 2\left(-\overline{\psi}\cos{\mu a} + d_0\sin{\mu a} \right) \sum_{n=1}^{\infty} (-1)^n J_{2n} \left( \mu a \alpha \right) &\cos\left( \frac{2nmy}{a} \right) \\
        + 2\left(-\overline{\psi}\sin{\mu a} - d_0\cos{\mu a} \right) \sum_{n=0}^{\infty}(-1)^{n}J_{2n+1}\left(\mu a \alpha \right)&\cos\left( \frac{(2n+1)my}{a}\right) \\
        +i \sum_{l=1}^{\infty} d_{lm}J_0\left( k_x^{(l)} a \alpha \right)\sin\left( k_x^{(l)} a \right) &\cos\left( \frac{lmy}{a} \right) \\
        +i \sum_{l=1}^{\infty} d_{lm}\sin\left( k_x^{(l)} a \right) \sum_{n=1}^{\infty} (-1)^n J_{2n} \left( k_x^{(l)} a \alpha \right) &\cos\left( \frac{(2n+l)my}{a} \right) \\
        +i \sum_{l=1}^{\infty} d_{lm}\sin\left( k_x^{(l)} a \right) \sum_{n=1}^{\infty} (-1)^n J_{2n} \left( k_x^{(l)} a \alpha \right) &\cos\left( \frac{(2n-l)my}{a} \right) \\
        -i \sum_{l=1}^{\infty} d_{lm}\cos\left( k_x^{(l)} a \right) \sum_{n=0}^{\infty}(-1)^{n}J_{2n+1}\left( k_x^{(l)  } a \alpha \right)&\cos\left( \frac{(2n+l+1)my}{a}\right) \\
        -i \sum_{l=1}^{\infty} d_{lm}\cos\left( k_x^{(l)} a \right) \sum_{n=0}^{\infty}(-1)^{n}J_{2n+1}\left( k_x^{(l)  } a \alpha \right)&\cos\left( \frac{(2n-l+1)my}{a}\right) \\
    \end{split}
\end{equation} 

Applying the Boundary Condition from (56a) in the Dewar paper,
\begin{equation}
    \begin{split}
        \hat{\psi}(x=x_{bdy}(y),y)&=\psi_a -\overline{\psi} -\overline{F}\psi_U(x=x_{bdy}(y)|\mu) \\
                                  &=\psi_a -\overline{\psi} -\frac{\overline{F}}{\mu} \\
                                  &+\frac{\overline{F}}{\mu}\cos\left( \mu a \right) \left[ J_0(\mu a \alpha) + 2\sum_{n=1}^{\infty} (-1)^n J_{2n}(\mu a \alpha) \cos\left( \frac{2nmy}{a} \right)\right] \\
                                  &+\frac{\overline{F}}{\mu}\sin\left( \mu a \right) \left[2 \sum_{n=0}^{\infty} (-1)^n J_{2n+1}(\mu a \alpha) \cos\left(\frac{(2n+1)my}{a}\right)\right]
    \end{split}
\end{equation} 

\section{Rearranged Series Solution Form}
For compactness, let
\begin{equation}
    A_{l' n}=\sin\left( k_x^{(l)} a \right) (-1)^n J_{2n}\left( k_x^{(l)}a\alpha \right) 
\end{equation} 
\begin{equation}
    B_{l' n}=\cos\left( k_x^{(l)}a \right) (-1)^n J_{2n+1}\left( k_x^{(l)}a\alpha \right) 
\end{equation} 
\begin{equation}
    C_{l' n}=\cos\left( k_x^{(l)} a \right) (-1)^n J_{2n}\left( k_x^{(l)}a\alpha \right) 
\end{equation} 
\begin{equation}
    D_{l' n}=\sin\left( k_x^{(l)}a \right) (-1)^n J_{2n+1}\left( k_x^{(l)}a\alpha \right) 
\end{equation} 

With these conventions in place, the solution can be rearranged as
\begin{equation}
    \begin{split}
        \hat{\psi}\left( x=x_{\text{bdy}}(y), y \right) &= \\
                                                        &-\overline{\psi} \sum_{n=0}^{\infty} C_{l'=0,n} \left[\cos\left( \frac{(2n+l)my}{a} \right) + \cos\left( \frac{(2n-l)my}{a} \right) \right]_{l=0} \\
                                                        &+\overline{\psi} C_{l'=0,n=0} \\
                                                        &-\overline{\psi} \sum_{n=0}^{\infty} D_{l'=0,n} \left[\cos\left( \frac{(2n+l+1)my}{a} \right) + \cos\left( \frac{(2n-l+1)my}{a} \right) \right]_{l=0} \\
                                                        &+\sum_{l=0}^{\infty} \sum_{n=0}^{\infty} d_{l'} A_{l' n} \left[\cos\left( \frac{(2n+l)my}{a} \right) + \cos\left( \frac{(2n-l)my}{a} \right) \right] \\
                                                        &-\sum_{l=0}^{\infty} d_{l'} A_{l',n=0} \left[\cos\left( \frac{(2n+l)my}{a} \right) + \cos\left( \frac{(2n-l)my}{a} \right) \right] \\
                                                        &+\sum_{l=0}^{\infty} \sum_{n=0}^{\infty} d_{l'} B_{l' n} \left[\cos\left( \frac{(2n+l+1)my}{a} \right) + \cos\left( \frac{(2n-l+1)my}{a} \right) \right]
    \end{split}
\end{equation} 

with the RH side as
\begin{equation}
    \begin{split}
        \psi_a -\overline{\psi} -\overline{F}\psi_U(x=x_{bdy}(y)|\mu)&= \\
                                                                     &= \psi_a - \overline{\psi} - \frac{\overline{F}}{\mu} \\
                                                                     &+ \frac{\overline{F}}{\mu} \sum_{n=0}^{\infty} C_{l'=0,n} \left[\cos\left( \frac{(2n+l)my}{a} \right) + \cos\left( \frac{(2n-l)my}{a} \right) \right]_{l=0} \\
                                                                     &- \frac{\overline{F}}{\mu} C_{l'=0,n=0} \\
                                                                     &+ \frac{\overline{F}}{\mu} \sum_{n=0}^{\infty} D_{l'=0,n} \left[\cos\left( \frac{(2n+l+1)my}{a} \right) + \cos\left( \frac{(2n-l+1)my}{a} \right) \right]_{l=0}
    \end{split}
\end{equation} 
\end{document}
